ambient_capabilities_coq_model/assert.v
@@ -85,26 +85,26 @@ Module Assert.
                            sat M σ A2 ->
                            sat M σ (A1 ∧ A2)
 
-  | sat_or1 : forall M σ A1 A2, sat M σ A1 ->
-                           sat M σ (A1 ∨ A2)
+(*  | sat_or1 : forall M σ A1 A2, sat M σ A1 ->
+                           sat M σ (A1 ∨ A2)*)
 
-  | sat_or2 : forall M σ A1 A2, sat M σ A2 ->
-                           sat M σ (A1 ∨ A2)
+(*  | sat_or2 : forall M σ A1 A2, sat M σ A2 ->
+                           sat M σ (A1 ∨ A2)*)
 
   | sat_neg : forall M σ A, nsat M σ A ->
                        sat M σ (¬ A)
 
   | sat_all : forall M σ C A, (forall α, glob_reachable α σ ->
-                               eval M σ (e_class (e_val (v_addr α)) C) v_true ->
+                               eval M σ (e_typ (e_val (v_addr α)) (t_cls C)) v_true ->
                                sat M σ ([α /s 0] A)) ->
                          sat M σ (a_all C A)
 
   | sat_ex : forall M σ α C A, glob_reachable α σ ->
                           sat M σ ([α /s 0] A) ->
-                          sat M σ (a_exp (e_class (e_val (v_addr α)) C)) ->
+                          sat M σ (a_exp (e_typ (e_val (v_addr α)) (t_cls C))) ->
                           sat M σ (a_ex C A)
 
-  | sat_extl : forall M σ e C, sat M σ (a_exp (e_class e C)) ->
+  | sat_extl : forall M σ e C, sat M σ (a_exp (e_typ e (t_cls C))) ->
                           ~ C ∈ snd M ->
                           sat M σ (a_extl e)
 
@@ -162,24 +162,24 @@ The above relies on the fact that "this" is always in the local variable map
   | nsat_and2 : forall M σ A1 A2, nsat M σ A2 ->
                              nsat M σ (A1 ∧ A2)
 
-  | nsat_or : forall M σ A1 A2, nsat M σ A1 ->
+(*  | nsat_or : forall M σ A1 A2, nsat M σ A1 ->
                            nsat M σ A2 ->
-                           nsat M σ (A1 ∨ A2)
+                           nsat M σ (A1 ∨ A2)*)
 
-  | nsat_neg : forall M σ A, sat M σ A ->
-                        nsat M σ (¬ A)
+(*  | nsat_neg : forall M σ A, sat M σ A ->
+                        nsat M σ (¬ A)*)
 
   | nsat_all : forall M σ α C A, glob_reachable α σ ->
-                            sat M σ (a_exp (e_class (e_val (v_addr α)) C)) ->
+                            sat M σ (a_exp (e_typ (e_val (v_addr α)) (t_cls C))) ->
                             nsat M σ ([α /s 0] A) ->
                             nsat M σ (a_all C A)
 
   | nsat_ex : forall M σ C A, (forall α, glob_reachable α σ ->
-                               eval M σ (e_class (e_val (v_addr α)) C) v_true ->
+                               eval M σ (e_typ (e_val (v_addr α)) (t_cls C)) v_true ->
                                nsat M σ ([α /s 0] A)) ->
                          nsat M σ (a_ex C A)
 
-  | nsat_extl : forall M σ e C, sat M σ (a_exp (e_class e C)) ->
+  | nsat_extl : forall M σ e C, sat M σ (a_exp (e_typ e (t_cls C))) ->
                            C ∈ snd M ->
                            nsat M σ (a_extl e)
 
